pcuic/theories/PCUICLiftSubst.v
@@ -221,7 +221,7 @@ Qed.
 Hint Resolve -> on_snd_eq_id_spec : all.
 Hint Resolve -> on_snd_eq_spec : all.
 
-Lemma map_def_eq_spec {A B : Set} (f f' g g' : A -> B) (x : def A) :
+Lemma map_def_eq_spec {A B} (f f' g g' : A -> B) (x : def A) :
   f (dtype x) = g (dtype x) ->
   f' (dbody x) = g' (dbody x) ->
   map_def f f' x = map_def g g' x.
@@ -230,7 +230,7 @@ Proof.
 Qed.
 Hint Resolve map_def_eq_spec : all.
 
-Lemma map_def_id_spec {A : Set} (f f' : A -> A) (x : def A) :
+Lemma map_def_id_spec {A} (f f' : A -> A) (x : def A) :
   f (dtype x) = (dtype x) ->
   f' (dbody x) = (dbody x) ->
   map_def f f' x = x.
